Compiler/CompilationModel/ValidationInterop.lean
@@ -86,6 +86,9 @@ def validateInteropExpr (context : String) : Expr → Except String Unit
   | Expr.arrayElement _ index | Expr.arrayElementWord _ index _ _ | Expr.arrayElementDynamicWord _ index _
   | Expr.arrayElementDynamicMemberLength _ index _ =>
       validateInteropExpr context index
+  | Expr.arrayElementDynamicMemberElement _ index _ innerIndex => do
+      validateInteropExpr context index
+      validateInteropExpr context innerIndex
   | Expr.add a b | Expr.sub a b | Expr.mul a b | Expr.div a b | Expr.sdiv a b | Expr.mod a b | Expr.smod a b |
     Expr.bitAnd a b | Expr.bitOr a b | Expr.bitXor a b | Expr.shl a b | Expr.shr a b |
     Expr.sar a b | Expr.signextend a b |
